ulib/FStar.TSet.fst
@@ -110,7 +110,6 @@ let lemma_equal_refl  #a s1 s2 = ()
 abstract let tset_of_set (#a:eqtype) (s:Set.set a) :set a =
   fun (x:a) -> squash (b2t (Set.mem x s))
 
-#set-options "--debug FStar.TSet --debug_level Extreme --print_effect_args --print_bound_var_types --ugly --print_implicits --debug_level Rel --debug_level RelCheck"
 private let lemma_mem_tset_of_set_l (#a:eqtype) (s:Set.set a) (x:a)
   :Lemma (requires True)
          (ensures (mem x (tset_of_set s) ==> Set.mem x s))
@@ -123,49 +122,49 @@ private let lemma_mem_tset_of_set_l (#a:eqtype) (s:Set.set a) (x:a)
       FStar.Squash.give_proof u
     else ()
 
-// private let lemma_mem_tset_of_set_r (#a:eqtype) (s:Set.set a) (x:a)
-//   :Lemma (requires True)
-//          (ensures (Set.mem x s ==> mem x (tset_of_set s)))
-//   = if Set.mem x s then
-//       let u:squash (b2t (Set.mem x s)) = () in
-//       let _ = assert (mem x (tset_of_set s) == squash (b2t (Set.mem x s))) in
-//       FStar.Squash.give_proof u
-//     else ()
+private let lemma_mem_tset_of_set_r (#a:eqtype) (s:Set.set a) (x:a)
+  :Lemma (requires True)
+         (ensures (Set.mem x s ==> mem x (tset_of_set s)))
+  = if Set.mem x s then
+      let u:squash (b2t (Set.mem x s)) = () in
+      let _ = assert (mem x (tset_of_set s) == squash (b2t (Set.mem x s))) in
+      FStar.Squash.give_proof u
+    else ()
 
-// let lemma_mem_tset_of_set (#a:eqtype) (s:Set.set a) (x:a)
-//   :Lemma (requires True)
-//          (ensures  (Set.mem x s <==> mem x (tset_of_set s)))
-//          [SMTPat (mem x (tset_of_set s))]
-//   = lemma_mem_tset_of_set_l #a s x; lemma_mem_tset_of_set_r #a s x
+let lemma_mem_tset_of_set (#a:eqtype) (s:Set.set a) (x:a)
+  :Lemma (requires True)
+         (ensures  (Set.mem x s <==> mem x (tset_of_set s)))
+         [SMTPat (mem x (tset_of_set s))]
+  = lemma_mem_tset_of_set_l #a s x; lemma_mem_tset_of_set_r #a s x
 
-// abstract
-// let filter (#a:Type) (f:a -> Type0) (s:set a) : set a =
-//   (fun (x:a) -> f x /\ s x)
+abstract
+let filter (#a:Type) (f:a -> Type0) (s:set a) : set a =
+  (fun (x:a) -> f x /\ s x)
 
-// let lemma_mem_filter (#a:Type) (f:(a -> Type0)) (s:set a) (x:a)
-//   :Lemma (requires True)
-//          (ensures  (mem x (filter f s) <==> mem x s /\ f x))
-//          [SMTPat (mem x (filter f s))]
-//   = ()
+let lemma_mem_filter (#a:Type) (f:(a -> Type0)) (s:set a) (x:a)
+  :Lemma (requires True)
+         (ensures  (mem x (filter f s) <==> mem x s /\ f x))
+         [SMTPat (mem x (filter f s))]
+  = ()
 
-// let exists_y_in_s (#a:Type) (#b:Type) (s:set a) (f:a -> Tot b) (x:b) : Tot prop =
-//  exists (y:a). mem y s /\ x == f y
+let exists_y_in_s (#a:Type) (#b:Type) (s:set a) (f:a -> Tot b) (x:b) : Tot prop =
+ exists (y:a). mem y s /\ x == f y
 
-// abstract
-// let map (#a:Type) (#b:Type) (f:a -> Tot b) (s:set a) : Tot (set b) = exists_y_in_s s f
+abstract
+let map (#a:Type) (#b:Type) (f:a -> Tot b) (s:set a) : Tot (set b) = exists_y_in_s s f
 
-// let lemma_mem_map (#a:Type) (#b:Type) (f:(a -> Tot b)) (s:set a) (x:b)
-//   :Lemma ((exists (y:a). {:pattern (mem y s)} mem y s /\ x == f y) <==> mem x (map f s))
-//          [SMTPat (mem x (map f s))]
-//   = ()
+let lemma_mem_map (#a:Type) (#b:Type) (f:(a -> Tot b)) (s:set a) (x:b)
+  :Lemma ((exists (y:a). {:pattern (mem y s)} mem y s /\ x == f y) <==> mem x (map f s))
+         [SMTPat (mem x (map f s))]
+  = ()
 
-// #reset-options
-// val as_set': #a:Type -> list a -> Tot (set a)
-// let rec as_set' #a l =
-//   match l with
-//   | [] -> empty
-//   | hd::tl -> union (singleton hd) (as_set' tl)
+#reset-options
+val as_set': #a:Type -> list a -> Tot (set a)
+let rec as_set' #a l =
+  match l with
+  | [] -> empty
+  | hd::tl -> union (singleton hd) (as_set' tl)
 
 
-// (* unfold let as_set (#a:Type) (l:list a) : set a = *)
-// (*   Prims.norm [zeta; iota; delta_only ["FStar.TSet.as_set'"]] (as_set' l) *)
+(* unfold let as_set (#a:Type) (l:list a) : set a = *)
+(*   Prims.norm [zeta; iota; delta_only ["FStar.TSet.as_set'"]] (as_set' l) *)
